coq/ZF/Meta/Test/Decl/Class/Equiv.v
@@ -2,9 +2,9 @@ Require Import Coq.Lists.List.
 Require Import Coq.Strings.String.
 
 Require Import ZF.Meta.Ctx.
-Require Import ZF.Meta.Decl.
+Require Import ZF.Meta.DeclTerm.
 Require Import ZF.Meta.Env.
-Require Import ZF.Meta.HasTyDecl.
+Require Import ZF.Meta.HasTyDeclTerm.
 Require Import ZF.Meta.HasTy.
 Require Import ZF.Meta.HasTyIn.
 Require Import ZF.Meta.Term.
@@ -15,13 +15,13 @@ Import ListNotations.
 (* Declarations.                                                                *)
 
 (* Definition toClass (a:U) : Class := fun x => x :< a.                         *)
-Definition toClass : Decl :=
+Definition toClass : DeclTerm :=
   {| para := [TySet];
      res  := TyClass;
      body := Some (Lam (Elem (Var 0) (Var 1))) |}.
 
 (* Definition equiv (P Q:Class) : Prop := forall x, P x <-> Q x.                *)
-Definition equiv : Decl :=
+Definition equiv : DeclTerm :=
   {| para := [TyClass; TyClass];
      res  := TyProp;
      body := Some
@@ -39,14 +39,14 @@ Definition env : Env := Env.fromList
 (* Body checks.                                                                 *)
 
 (* The declaration body for toClass maps a set to its membership class.         *)
-Proposition toClassCheckBody : HasTyDecl Env.empty toClass.
+Proposition toClassCheckBody : HasTyDeclTerm Env.empty toClass.
 Proof.
   (* Proof by Hermes + gpt 5.5                                                  *)
   apply HasTyLam, HasTyElem; apply (HasTyVar _ _ _ TySet); reflexivity.
 Qed.
 
 (* The declaration body for equivalence compares two classes pointwise.         *)
-Proposition equivCheckBody : HasTyDecl Env.empty equiv.
+Proposition equivCheckBody : HasTyDeclTerm Env.empty equiv.
 Proof.
   (* Proof by Hermes + gpt 5.5                                                  *)
   apply HasTyAll, HasTyIff.
