coq/ZF/Meta/HasTyDeclTerm.v
@@ -1,0 +1,10 @@
+Require Import ZF.Meta.DeclTerm.
+Require Import ZF.Meta.Env.
+Require Import ZF.Meta.HasTy.
+
+(* A term declaration is well typed when its body has its declared sort.        *)
+Definition HasTyDeclTerm (e:Env) (d:DeclTerm) : Prop :=
+  match DeclTerm.body d with
+  | Some t => HasTy (Env.toSigs e) (DeclTerm.ctx d) t (DeclTerm.res d)
+  | None   => True
+  end.
